TLB_PDC/ARMv7A_Mem_Write_Read_Ref.thy
@@ -187,11 +187,11 @@ lemma mmu_write_incon_set_rel:
       apply blast
      apply (clarsimp simp: pt_walk_new_fault_pt_walk_fault)
     apply (erule disjE)
-     apply (subgoal_tac "the (pt_walk (ASID r) (MEM q) (TTBR0 r) xc) = the (pt_walk (ASID r) (MEM s) (TTBR0 r) x)")
+     apply (subgoal_tac "the (pt_walk (ASID r) (MEM q) (TTBR0 r) xb) = the (pt_walk (ASID r) (MEM s) (TTBR0 r) x)")
       apply (case_tac "\<not> is_fault (pt_walk (ASID r) (MEM s) (TTBR0 r) x)")
-  using saturatd_lookup_hit_no_fault apply fastforce
+       using saturatd_lookup_hit_no_fault apply fastforce
       apply blast
-     apply (subgoal_tac "the (pt_walk (ASID r) (MEM q) (TTBR0 r) xc) = the (pt_walk (ASID r) (MEM q) (TTBR0 r) x)")
+     apply (subgoal_tac "the (pt_walk (ASID r) (MEM q) (TTBR0 r) xb) = the (pt_walk (ASID r) (MEM q) (TTBR0 r) x)")
       apply (drule pt_walk_new_equal_pt_walk, simp add: is_fault_def)
      apply (frule  asid_tlb_lookup_range_fault_pt_walk)
      apply (drule_tac x = x in bspec; clarsimp simp: lookup_asid_tlb_hit_entry_range)
@@ -210,9 +210,9 @@ lemma mmu_write_incon_set_rel:
      apply blast
     apply (clarsimp simp: pt_walk_new_fault_pde_walk_fault)
    apply (erule disjE)
-    apply (subgoal_tac "the (pdc_walk (ASID r) (MEM q) (TTBR0 r) xc) = the (pdc_walk (ASID r) (MEM s) (TTBR0 r) x)")
+    apply (subgoal_tac "the (pdc_walk (ASID r) (MEM q) (TTBR0 r) xb) = the (pdc_walk (ASID r) (MEM s) (TTBR0 r) x)")
      prefer 2
-     apply (subgoal_tac "the (pdc_walk (ASID r) (MEM q) (TTBR0 r) xc) = the (pdc_walk (ASID r) (MEM q) (TTBR0 r) x)")
+     apply (subgoal_tac "the (pdc_walk (ASID r) (MEM q) (TTBR0 r) xb) = the (pdc_walk (ASID r) (MEM q) (TTBR0 r) x)")
       apply clarsimp
       apply (drule pt_walk_new_equal_pdc_walk, simp add: is_fault_def)
      apply (frule lookup_pdc_range_fault_pt_walk)
@@ -221,11 +221,11 @@ lemma mmu_write_incon_set_rel:
       apply clarsimp
   using saturatd_lookup_pdc_hit_no_fault apply fastforce
   apply blast
-  apply (subgoal_tac "the(pdc_walk (ASID r) (MEM q) (TTBR0 r) xc) = the(pdc_walk (ASID r) (MEM s) (TTBR0 r) x)" )
+  apply (subgoal_tac "the(pdc_walk (ASID r) (MEM q) (TTBR0 r) xb) = the(pdc_walk (ASID r) (MEM s) (TTBR0 r) x)" )
   apply (case_tac "is_fault (pdc_walk (ASID r) (MEM s) (TTBR0 r) x)")
   apply blast
   using saturatd_lookup_pdc_hit_no_fault apply fastforce
-  apply (subgoal_tac " the (pdc_walk (ASID r) (MEM q) (TTBR0 r) xc) =  the(pdc_walk (ASID r) (MEM q) (TTBR0 r) x)")
+  apply (subgoal_tac " the (pdc_walk (ASID r) (MEM q) (TTBR0 r) xb) =  the(pdc_walk (ASID r) (MEM q) (TTBR0 r) x)")
     apply clarsimp
     apply (simp add: pt_walk_partial_full_pdc_walk_eq)
    apply (meson lookup_asid_pdc_hit_entry_range lookup_pdc_range_fault_pt_walk 
@@ -325,8 +325,6 @@ lemma mmu_write_sat_incon_refine:
   by (rule lookup_non_global_union_asid_unequal_pdc, simp)
 
 
-
-   
 
 
 (* refinement for read theroems *)
@@ -457,7 +455,6 @@ lemma  mem_read1_consistent_tlb_rel_incon:
   apply (clarsimp simp: tlb_rel_abs_def state.defs)
   done
 
-find_consts "'a option set \<Rightarrow> 'a option"
 
 lemma mmu_read_sat_incon_rel_con:
   "\<lbrakk> mmu_read_size (va, sz) s = (val, s'); tlb_rel_abs (typ_sat_tlb s) (typ_set_tlb t);
