ROOT
@@ -2,10 +2,8 @@ chapter AFP
 
 session Word_Lib (AFP) in "Word_Lib" = "HOL-Word" +
   options [timeout = 300]
-  theories [document = false]
-    "HOL-Word.WordBitwise"
-    "HOL-Library.Prefix_Order"
-  theories 
+  sessions "HOL-Library"
+  theories
     Word_Lemmas_32
     Word_Lemmas_64
   document_files
@@ -13,17 +11,17 @@ session Word_Lib (AFP) in "Word_Lib" = "HOL-Word" +
 
 chapter TLB
 
-   
+
 session L3_LIBJ = Word_Lib +
   theories
     "L3_Library/L3_Lib"
 
-   
+
 session PTABLE_TLBJ = L3_LIBJ +
   theories
     "Page_Tables/PageTable_seL4"
 
-	
+
 
 session TLBJ = PTABLE_TLBJ +
   theories
@@ -40,7 +38,7 @@ session TLB_PDC_REFJ = TLB_ASID_REFJ +
   theories
     "TLB_PDC/Paper_Defs_machine_Inter"
     "Logic/Page_Table_Ops"
-    
+
 (*session CASE_STUDYJJ = TLB_ASID_REFJ +
   theories
     "Case_Study/Page_Table_Ops"
